examples/test5.smt2
@@ -1,4 +1,5 @@
 (set-logic UFLIA)
-(assert (not (or true false)))
+(declare-fun op_0 () Bool)
+(assert (not (or op_0 (not op_0))))
 (check-sat)
 (exit)
