examples/test6.smt2
@@ -1,5 +1,0 @@
-(set-logic UFLIA)
-(declare-fun op_0 () Bool)
-(assert (not (or op_0 (not op_0))))
-(check-sat)
-(exit)
